Changed the parametrized string manipulation strategies; fifo <<== nativeFifo wip

examples/NativeFifo.v
@@ -35,44 +35,46 @@ Section NativeFifo.
     end.
 
   (* defined methods *)
-  Definition enq {ty} : forall (d: ty dType), ActionT ty Void := fun d =>
+  Definition nativeEnq {ty} : forall (d: ty dType), ActionT ty Void := fun d =>
     (ReadN elt : listEltK ty <- ^"elt";
      Assert !$$(listIsFull elt);
      Write ^"elt" <- (Var _ (listEltK ty) (listEnq d elt));
      Retv)%kami.
 
-  Definition deq {ty} : ActionT ty dType :=
+  Definition nativeDeq {ty} : ActionT ty dType :=
     (ReadN elt : listEltK ty <- ^"elt";
      Assert !$$(listIsEmpty elt);
      Write ^"elt" <- (Var _ (listEltK ty) (listDeq elt));
      Ret (listFirstElt elt))%kami.
 
-  Definition firstElt {ty} : ActionT ty dType :=
+  Definition nativeFirstElt {ty} : ActionT ty dType :=
     (ReadN elt : listEltK ty <- ^"elt";
      Assert !$$(listIsEmpty elt);
      Ret (listFirstElt elt))%kami.
 
-  Definition fifo := MODULE {
+  Definition nativeFifo := MODULE {
     RegisterN ^"elt" : listEltK type <- (NativeConst nil nil)
 
-    with Method ^"enq"(d : dType) : Void := (enq d)
-    with Method ^"deq"() : dType := deq
-    with Method ^"firstElt"() : dType := firstElt
+    with Method ^"enq"(d : dType) : Void := (nativeEnq d)
+    with Method ^"deq"() : dType := nativeDeq
+    with Method ^"firstElt"() : dType := nativeFirstElt
   }.
 
-  Definition simpleFifo := MODULE {
+  Definition nativeSimpleFifo := MODULE {
     RegisterN ^"elt" : listEltK type <- (NativeConst nil nil)
 
-    with Method ^"enq"(d : dType) : Void := (enq d)
-    with Method ^"deq"() : dType := deq
+    with Method ^"enq"(d : dType) : Void := (nativeEnq d)
+    with Method ^"deq"() : dType := nativeDeq
   }.
 
 End NativeFifo.
 
-Hint Unfold fifo simpleFifo : ModuleDefs.
-Hint Unfold enq deq : MethDefs.
+Hint Unfold nativeFifo nativeSimpleFifo : ModuleDefs.
+Hint Unfold listEltT listEltK listElt
+     listIsFull listIsEmpty listEnq listDeq listFirstElt
+     nativeEnq nativeDeq nativeFirstElt: MethDefs.
 
-Require Import Refinement.
+Require Import Refinement Decomposition Tactics Lib.FMap.
 
 Section Facts.
   Variable fifoName: string.
@@ -80,12 +82,92 @@ Section Facts.
   Variable dType: Kind.
   Variable default: ConstT dType.
 
-  Definition realFifo := Fifo.fifo fifoName sz dType.
-  Definition nativeFifo := @fifo fifoName sz dType default.
+  Definition fifo := fifo fifoName sz dType.
+  Definition nfifo := @nativeFifo fifoName sz dType default.
 
-  Lemma fifo_refines_nativefifo: realFifo <<== nativeFifo.
+  Notation "^ s" := (fifoName .. s) (at level 0).
+
+  Fixpoint fifo_nfifo_elt_not_full
+           (eltv : word sz -> type dType)
+           (enqPv : word sz)
+           (edSub : nat): list (type dType) :=
+    match edSub with
+    | O => nil
+    | S ed =>
+      (eltv (enqPv ^- (natToWord sz edSub)))
+        :: (fifo_nfifo_elt_not_full eltv enqPv ed)
+    end.
+
+  Definition fifo_nfifo_regMap (r: RegsT): RegsT.
+  Proof.
+    kgetv ^"elt"%string eltv r (Vector dType sz) (M.empty (sigT (fullType type))).
+    kgetv ^"full"%string fullv r Bool (M.empty (sigT (fullType type))).
+    kgetv ^"enqP"%string enqPv r (Bit sz) (M.empty (sigT (fullType type))).
+    kgetv ^"deqP"%string deqPv r (Bit sz) (M.empty (sigT (fullType type))).
+
+    refine (M.add ^"elt" (existT _ (listEltK dType type) _) (M.empty _)).
+    destruct (weq enqPv deqPv).
+    - refine (if fullv then _ else _).
+      + exact ((eltv deqPv) :: (fifo_nfifo_elt_not_full eltv enqPv (wordToNat (wones sz)))).
+      + exact nil.
+    - exact (fifo_nfifo_elt_not_full eltv enqPv (wordToNat (enqPv ^- deqPv))).
+  Defined.
+  Hint Unfold fifo_nfifo_regMap: MethDefs.
+  
+  Definition fifo_nfifo_ruleMap (_: RegsT) (r: string): option string := Some r.
+  Hint Unfold fifo_nfifo_ruleMap: MethDefs.
+
+  Definition fifo_nfifo_labelMap (_: string) (s: sigT SignT): option (sigT SignT) := Some s.
+
+  Definition fifo_nfifo_substepRuleMap:
+    forall (oImp : RegsT) (uImp : UpdatesT)
+           (rule : string) (csImp : MethsT),
+      reachable oImp fifo ->
+      Substep fifo oImp uImp (Rle (Some rule))
+              csImp ->
+      {uSpec : UpdatesT |
+       Substep nfifo (fifo_nfifo_regMap oImp) uSpec
+               (Rle (fifo_nfifo_ruleMap oImp rule))
+               (liftToMap1 fifo_nfifo_labelMap csImp) /\
+       (forall o : RegsT,
+           M.union uSpec (fifo_nfifo_regMap o) =
+           fifo_nfifo_regMap (M.union uImp o))}.
   Proof.
     admit.
+  Qed.
+  
+  Definition fifo_nfifo_substepMethMap:
+    forall (oImp : RegsT) (uImp : UpdatesT)
+           (meth : Struct.Attribute (sigT SignT))
+           (csImp : MethsT),
+      reachable oImp fifo ->
+      Substep fifo oImp uImp (Meth (Some meth))
+              csImp ->
+      {uSpec : UpdatesT |
+       Substep nfifo (fifo_nfifo_regMap oImp) uSpec
+               (Meth (liftP fifo_nfifo_labelMap meth))
+               (liftToMap1 fifo_nfifo_labelMap csImp) /\
+       (forall o : RegsT,
+           M.union uSpec (fifo_nfifo_regMap o) =
+           fifo_nfifo_regMap (M.union uImp o))}.
+  Proof.
+    admit.
+  Qed.
+
+  Lemma fifo_refines_nativefifo: fifo <<== nfifo.
+  Proof.
+    apply decomposition with
+    (theta:= fifo_nfifo_regMap)
+      (ruleMap:= fifo_nfifo_ruleMap)
+      (substepRuleMap:= fifo_nfifo_substepRuleMap)
+      (substepMethMap:= fifo_nfifo_substepMethMap).
+
+    - kdecompose_regmap_init.
+      kinv_finish.
+    - auto.
+    - auto.
+    - admit.
+    - kequiv.
   Qed.
 
 End Facts.
