lib/Indexer.v
@@ -1,22 +1,9 @@
-Require Import Bool Ascii String List Eqdep Omega.
+Require Import Bool Ascii String Eqdep Omega.
 Require Import CommonTactics.
 
 (** Some string manipulation lemmas *)
 
-Lemma prepend_same: forall x a b, (x ++ a)%string = (x ++ b)%string -> a = b.
-Proof.
-  induction x; intros; intuition.
-  inv H; auto.
-Qed.
-
-Lemma substring_append_1:
-  forall s1 s2 n,
-    substring (String.length s1) n (s1 ++ s2) = substring 0 n s2.
-Proof. induction s1; simpl; intros; auto. Qed.
-
-Lemma substring_empty:
-  forall s, substring 0 0 s = ""%string.
-Proof. induction s; simpl; intros; auto. Qed.
+Open Scope string_scope.
 
 Lemma string_append_assoc:
   forall {a b c : string}, (a ++ b ++ c)%string = ((a ++ b) ++ c)%string.
@@ -26,6 +13,104 @@ Proof.
   simpl. reflexivity.
   simpl. rewrite IHa. reflexivity.
 Qed.
+
+Lemma append_length:
+  forall s1 s2,
+    length (s1 ++ s2) = length s1 + length s2.
+Proof. induction s1; simpl; intros; auto. Qed.
+
+Lemma prepend_same: forall x a b, x ++ a = x ++ b -> a = b.
+Proof.
+  induction x; intros; intuition.
+  inv H; auto.
+Qed.
+
+Lemma append_empty: forall s, s ++ "" = s.
+Proof.
+  induction s; simpl; intros; auto.
+  f_equal; auto.
+Qed.
+
+Fixpoint string_rev (s: string) :=
+  match s with
+  | EmptyString => EmptyString
+  | String a s' => ((string_rev s') ++ (String a EmptyString))%string
+  end.
+
+Lemma string_rev_empty:
+  forall s, string_rev s = EmptyString -> s = EmptyString.
+Proof.
+  destruct s; simpl; intros; auto.
+  assert (length (string_rev s ++ String a "") = length "")
+    by (rewrite H; reflexivity).
+  rewrite append_length in H0; simpl in H0.
+  omega.
+Qed.
+
+Lemma string_append_same_singleton:
+  forall s1 s2 a1 a2,
+    s1 ++ String a1 "" = s2 ++ String a2 "" ->
+    s1 = s2 /\ a1 = a2.
+Proof.
+  induction s1; simpl; intros.
+  - destruct s2; simpl in *.
+    + inv H; auto.
+    + inv H; destruct s2; inv H2.
+  - destruct s2; simpl in *.
+    + exfalso.
+      assert (length (String a (s1 ++ String a1 "")) =
+              length (String a1 "")) by (rewrite H; reflexivity); clear H.
+      simpl in H0; rewrite append_length in H0; simpl in H0.
+      omega.
+    + inv H.
+      specialize (IHs1 _ _ _ H2); dest; subst; auto.
+Qed.
+
+Lemma string_rev_same:
+  forall s1 s2, string_rev s1 = string_rev s2 -> s1 = s2.
+Proof.
+  induction s1; simpl; intros.
+  - apply eq_sym, string_rev_empty in H; auto.
+  - destruct s2.
+    + simpl in H.
+      assert (length (string_rev s1 ++ String a "") = length "")
+        by (rewrite H; reflexivity).
+      rewrite append_length in H0; simpl in H0.
+      omega.
+    + simpl in H.
+      apply string_append_same_singleton in H; dest; subst.
+      f_equal; auto.
+Qed.
+
+Lemma string_rev_app:
+  forall s1 s2, string_rev (s1 ++ s2) = ((string_rev s2) ++ (string_rev s1))%string.
+Proof.
+  induction s1; simpl; intros.
+  - destruct s2; auto.
+    simpl; rewrite <-string_append_assoc; f_equal.
+  - destruct s2; simpl in *.
+    + rewrite append_empty; auto.
+    + rewrite IHs1; simpl.
+      rewrite string_append_assoc; auto.
+Qed.
+
+Lemma append_same: forall x a b, (a ++ x)%string = (b ++ x)%string -> a = b.
+Proof.
+  intros; apply string_rev_same.
+  assert (string_rev (a ++ x) = string_rev (b ++ x))
+    by (rewrite H; reflexivity).
+  do 2 rewrite string_rev_app in H0.
+  eapply prepend_same; eauto.
+Qed.
+    
+Lemma substring_append_1:
+  forall s1 s2 n,
+    substring (String.length s1) n (s1 ++ s2) = substring 0 n s2.
+Proof. induction s1; simpl; intros; auto. Qed.
+
+Lemma substring_empty:
+  forall s, substring 0 0 s = ""%string.
+Proof. induction s; simpl; intros; auto. Qed.
 
 (** End of string manipulation lemmas *)
 
@@ -42,18 +127,18 @@ Definition indexSymbol: string := "__"%string.
 Definition prefixSymbol: string := "."%string.
 
 Definition withIndex str idx := 
-  append (append (string_of_nat idx) indexSymbol) str.
+  append str (append indexSymbol (string_of_nat idx)).
 Definition withPrefix pre str :=
-  append (append pre prefixSymbol) str.
+  append str (append prefixSymbol pre).
 
 Theorem withIndex_eq : withIndex = fun str idx =>
-  append (append (string_of_nat idx) indexSymbol) str.
+  append str (append indexSymbol (string_of_nat idx)).
 Proof.
   reflexivity.
 Qed.
 
 Lemma string_of_nat_index_1:
-  forall i j, j <= i -> get j (string_of_nat i) = Some "a"%char.
+  forall i j, j <= i -> forall s, get j (string_of_nat i ++ s) = Some "a"%char.
 Proof.
   induction i; simpl; intros.
   - destruct j; try omega; auto.
@@ -62,35 +147,18 @@ Proof.
 Qed.
 
 Lemma string_of_nat_index_2:
-  forall i j, j > i -> get j (string_of_nat i) = None.
-Proof.
-  induction i; simpl; intros.
-  - destruct j; try omega; auto.
-  - destruct j; try omega; auto.
-    apply IHi; omega.
-Qed.
-
-Lemma append_length:
-  forall s1 s2,
-    String.length (s1 ++ s2) = String.length s1 + String.length s2.
-Proof. induction s1; simpl; intros; auto. Qed.
-
-Lemma withIndex_index_1:
-  forall s i j, j <= i -> get j (withIndex s i) = Some "a"%char.
-Proof.
-  unfold withIndex; intros.
-  rewrite <-append_correct1.
-  - rewrite <-append_correct1.
-    + apply string_of_nat_index_1; auto.
-    + rewrite string_of_nat_length; omega.
-  - rewrite append_length.
-    rewrite string_of_nat_length; omega.
-Qed.
-
-Lemma withIndex_index_2:
-  forall s i, get (S i) (withIndex s i) = Some "_"%char.
+  forall i s, get (S i) (string_of_nat i ++ s) = get 0 s.
 Proof.
   induction i; simpl; intros; auto.
+Qed.
+
+Lemma string_of_nat_rev:
+  forall i, string_rev (string_of_nat i) = string_of_nat i.
+Proof.
+  induction i; simpl; intros; auto.
+  rewrite IHi.
+  clear; induction i; auto.
+  simpl; f_equal; auto.
 Qed.
 
 Lemma withIndex_neq:
@@ -98,33 +166,35 @@ Lemma withIndex_neq:
     i <> j ->
     withIndex a i <> withIndex b j.
 Proof.
-  intros; destruct (gt_eq_gt_dec i j).
-  - destruct s.
-    + intro Hx.
-      assert (get (S i) (withIndex a i) = get (S i) (withIndex b j)) by (rewrite Hx; auto).
-      rewrite withIndex_index_2 with (i:= i) in H0 by omega.
-      rewrite withIndex_index_1 in H0 by omega.
-      inv H0.
-    + elim H; auto.
-  - intro Hx.
-    assert (get (S j) (withIndex a i) = get (S j) (withIndex b j)) by (rewrite Hx; auto).
-    rewrite withIndex_index_2 with (i:= j) in H0 by omega.
-    rewrite withIndex_index_1 in H0 by omega.
-    inv H0.
-Qed.
+  unfold withIndex; intros; intro Hx; elim H; clear H.
+  assert (string_rev (a ++ indexSymbol ++ string_of_nat i) =
+          string_rev (b ++ indexSymbol ++ string_of_nat j))
+    by (rewrite Hx; reflexivity); clear Hx.
+  repeat rewrite string_rev_app in H.
+  repeat rewrite string_of_nat_rev in H.
 
-Lemma withIndex_neq_prefix:
-  forall a b i j,
-    a <> b ->
-    withIndex a i <> withIndex b j.
-Proof.
-  intros; destruct (eq_nat_dec i j); [subst|].
-  - apply discr_var; auto.
-  - apply withIndex_neq; auto.
+  destruct (gt_eq_gt_dec i j); auto.
+  - destruct s; auto; exfalso.
+    simpl in H.
+    do 2 rewrite <-string_append_assoc in H.
+    match type of H with
+    | ?l = ?r => assert (get (S i) l = get (S i) r) by (rewrite H; reflexivity)
+    end; clear H.
+    rewrite string_of_nat_index_2 in H0; simpl in H0.
+    rewrite string_of_nat_index_1 in H0; inv H0; omega.
+  - exfalso; simpl in H.
+    do 2 rewrite <-string_append_assoc in H.
+    match type of H with
+    | ?l = ?r => assert (get (S j) l = get (S j) r) by (rewrite H; reflexivity)
+    end; clear H.
+    rewrite string_of_nat_index_2 in H0; simpl in H0.
+    rewrite string_of_nat_index_1 in H0; inv H0; omega.
 Qed.
 
 Global Opaque withIndex.
 
 Notation "str '__' idx" := (withIndex str idx) (at level 0).
 Notation "pre '..' str" := (withPrefix pre str) (at level 0).
-                           
+
+Close Scope string_scope.
+
